making server and client executable same so that clients can send closures over the network.

examples/wysteria/Runtime.ml
@@ -1,0 +1,30 @@
+module IO = Extlib.IO
+
+module Unix = BatUnix
+module Marshal = BatMarshal
+
+open AST
+
+type chan_in = IO.input
+type chan_out = unit IO.output
+
+let open_connection (port:int) :(chan_in * chan_out) =
+  let sock_addr = Unix.ADDR_INET (Unix.inet_addr_of_string "127.0.0.1", port) in
+  Unix.open_connection sock_addr
+
+let client_write (out:chan_out) (p:prin) (r:redex) :unit = Marshal.output out (p, r)
+let client_read (c_in:chan_in) :dvalue = Marshal.input c_in
+
+let establish_server (callback:chan_in -> chan_out -> unit) (port:int) =
+  let sock_addr = Unix.ADDR_INET (Unix.inet_addr_of_string "127.0.0.1", port) in
+  Unix.establish_server callback sock_addr
+
+let server_read (c:chan_in) :(prin * redex) = Marshal.input c
+let server_write (out:chan_out) (dv:dvalue) :unit = Marshal.output out dv
+let create_thread (f:unit -> unit) :unit = let _ = Thread.create f () in ()
+
+let is_server _ = Sys.argv.(1) = "0"
+let me _ = Sys.argv.(2)
+
+(* This is properly implemented in w-extraction branch *)
+let get_smc = fun _ -> Exp ((E_const C_unit), None)
