examples/wysteria/runtime.fsi
@@ -1,0 +1,29 @@
+(*--build-config
+   options:--admit_fsi FStar.Set --admit_fsi FStar.OrdSet --admit_fsi FStar.OrdMap;
+   variables:LIB=../../lib;
+   other-files:$LIB/set.fsi $LIB/heap.fst $LIB/st.fst $LIB/all.fst $LIB/ordset.fsi $LIB/ordmap.fsi ast.fst
+--*)
+
+
+module Runtime
+
+open AST
+
+type chan_in   // channel type to read input
+type chan_out  // channel type to send output
+
+val establish_server: callback:(chan_in -> chan_out -> ML unit) -> port:nat -> ML unit
+val server_read : chan_in  -> ML (prin * (r:redex{is_R_assec r /\ is_clos (R_assec.v r)}))
+val server_write: chan_out -> dvalue -> ML unit
+
+val open_connection : port:nat -> ML (chan_in * chan_out)
+val client_write: chan_out -> prin -> r:redex{is_R_assec r} -> ML unit
+val client_read : chan_in -> ML dvalue
+
+val create_thread: f:(unit -> ML unit) -> ML unit  // server spawns a new thread for each sec block
+
+val get_init_tenv : unit -> ML env
+
+val is_server: unit -> ML bool
+val me       : unit -> ML string
+val get_smc  : unit -> ML exp
