examples/wysteria/sinterpreter.fst
@@ -116,9 +116,6 @@ let step_correctness c =
   else if not (pre_assec c = NA) then C_assec_beta c c'
   else C_assec_ret c c'
 
-val is_terminal: config -> Tot bool
-let is_terminal (Conf _ _ s _ t) = s = [] && is_T_val t
-
 val step_star: config -> Dv (option config)
 let rec step_star c =
   if is_terminal c then Some c
